hmacdrbg/spec_hmac_drbg_pure_lemmas.v
@@ -1,18 +1,19 @@
 Require Import Coqlib.
 Require Import List. Import ListNotations.
 
-Require Import hmacdrbg.spec_hmac_drbg.
-Require Import hmacdrbg.HMAC256_DRBG_functional_prog.
+Require Import sha.general_lemmas. 
+Require Import sha.HMAC256_functional_prog.
+
+Require Import hmacdrbg.entropy.
 Require Import hmacdrbg.DRBG_functions.
 Require Import hmacdrbg.HMAC_DRBG_algorithms.
-Require Import hmacdrbg.entropy.
+Require Import hmacdrbg.HMAC256_DRBG_functional_prog.
+Require Import hmacdrbg.spec_hmac_drbg.
 (*Require Import sha.spec_hmacNK.
 Require Import sha.funspec_hmacNK.
-*)
+*)(*
 Require Import sha.spec_hmac.
-Require Import sha.protocol_spec_hmac.
-Require Import sha.general_lemmas.
-Require Import sha.HMAC256_functional_prog.
+Require Import sha.protocol_spec_hmac.*)
 
 Lemma isbyteZ_initialKey: Forall isbyteZ initial_key. 
 Proof. apply Forall_list_repeat; split; omega. Qed.
