hmacdrbg/verif_hmac_drbg_generate.v
@@ -1092,7 +1092,10 @@ Proof.
   { destruct additional; simpl in PNadditional; try contradiction.
     + subst i0; entailer.
     + rewrite da_emp_ptr. normalize.
-      unfold denote_tc_comparable. entailer.
+      unfold denote_tc_comparable. entailer!.
+      eapply derives_trans; try apply valid_pointer_weak.
+      apply sepcon_valid_pointer2. 
+      apply data_at_valid_ptr; trivial. apply top_share_nonidentity.
   }
   { forward. entailer!. subst after_reseed_add_len na.
     destruct should_reseed; simpl; trivial. rewrite andb_false_r. reflexivity.
