hmacdrbg/verif_mocked_md.v
@@ -11,7 +11,21 @@ Require Import hmacdrbg.spec_hmac_drbg.
 Axiom FINALNAME:_HMAC_Final = hmac._HMAC_Final. 
 Axiom UPDATENAME:_HMAC_Update = hmac._HMAC_Update. 
 Axiom INITNAME: _HMAC_Init = hmac._HMAC_Init. 
-Axiom CTX_Struct: Tstruct hmac_drbg._hmac_ctx_st noattr = spec_hmac.t_struct_hmac_ctx_st.
+Axiom CTX_Struct: Tstruct _hmac_ctx_st noattr = spec_hmac.t_struct_hmac_ctx_st.
+
+(*Axioms CS: hmac_drbg_compspecs.CompSpecs = spec_hmac.CompSpecs.*)
+
+Lemma body_md_free: semax_body HmacDrbgVarSpecs HmacDrbgFunSpecs
+       f_mbedtls_md_free md_free_spec.
+Proof.
+  start_function. (*
+  unfold UNDER_SPEC.EMPTY. rewrite <- CS.
+  assert_PROP(field_compatible spec_hmac.t_struct_hmac_ctx_st [] ctx) as FC by entailer.
+  rewrite data_at__isptr. Intros.
+  destruct ctx; try contradiction. clear Pctx.
+  unfold data_at_. unfold field_at_. simpl. 
+  rewrite field_at_data_at.*)
+Admitted. 
 
 Lemma body_md_get_size: semax_body HmacDrbgVarSpecs HmacDrbgFunSpecs
        f_mbedtls_md_get_size md_get_size_spec.
@@ -30,48 +44,23 @@ Proof.
   unfold_data_at 1%nat.
   forward. 
 
-  rewrite INITNAME, CTX_Struct.
-forward_call (r3, l, key, kv).
-Admitted. (*Probem: have two specs for hmac_init in context - for different scenarios!
-Locate f_mbedtls_md_hmac_starts.
-unfold UNDER_SPEC.EMPTY.
-assert ().
-(*Parameter hh:spec_hmac.hmacabs.*)
-  forward_call (r3, l, key(*map Vint (map Int.repr key)*), kv, b, i). , Zlength key, key, kv, hh).
-  Intros. normalize. (*FAIL*)
-  apply extract_exists_pre. intros vret. (*SUCCESS*)
- 
-  forward_if (PROP () LOCAL (temp _sha_ctx vret; temp _md_info info; 
-   temp _ctx c; temp _hmac h) 
-      SEP (memory_block Tsh (sizeof (Tstruct _hmac_ctx_st noattr)) vret;
-           data_at Tsh (Tstruct _mbedtls_md_context_t noattr) md_ctx c)).
-  { destruct (Memory.EqDec_val vret nullval).
-    + subst vret; entailer!.
-    + eapply derives_trans; try apply valid_pointer_weak.
-      apply sepcon_valid_pointer1.
-      apply memory_block_valid_ptr. apply top_share_nonidentity. omega.
-      entailer!. 
-  }
-  { (*null*) 
-    subst vret. simpl. forward.
-    Exists (-20864). entailer!. apply orp_right1. entailer!.
-  }
-  { destruct (eq_dec vret nullval); subst. elim H; trivial. clear n.
-    forward. entailer!.
-  }
-  rewrite memory_block_isptr. Intros.
-  unfold_data_at 1%nat.
-  forward. forward. Exists 0. entailer!. apply orp_right2.
-  Exists vret. unfold_data_at 1%nat. entailer!. 
+  rewrite INITNAME , CTX_Struct.
+  forward_call (@inr (val * Z * list Z * val) _ (r3, l, key, kv, b, i)).
+  (* call pattern for reset:
+  forward_call (@inl _ (val * Z * list Z * val * block * int) (r3, l, key, kv)).*)
+  { unfold spec_sha.data_block. normalize. cancel. }
+  forward.
+  cancel. unfold md_relate; simpl. cancel.
+  unfold spec_sha.data_block; normalize. cancel.
+  unfold_data_at 1%nat. cancel.
 Qed.
 
-*)
 Lemma body_md_update: semax_body HmacDrbgVarSpecs HmacDrbgFunSpecs
        f_mbedtls_md_hmac_update md_update_spec.
 Proof.
   start_function. 
   
-  unfold md_relate; unfold convert_abs.
+  unfold md_relate(*; unfold convert_abs*).
   destruct r as [r1 [r2 internal_r]].
   simpl.
   rewrite REP_isptr; Intros. 
@@ -83,7 +72,7 @@ Proof.
   rewrite data_at_isptr with (p:=d); Intros.
   destruct d; try contradiction.
 
-  rewrite UPDATENAME, CTX_Struct.  
+  rewrite UPDATENAME, CTX_Struct.
   forward_call (key, internal_r, Vptr b i, data, data1, kv).
   {
     unfold spec_sha.data_block.
@@ -95,7 +84,7 @@ Proof.
 
   (* prove the post condition *)
   unfold spec_sha.data_block.
-  unfold md_relate; unfold convert_abs.
+  unfold md_relate (*; unfold convert_abs*).
   entailer!.
 Qed.
 
@@ -104,7 +93,7 @@ Lemma body_md_final: semax_body HmacDrbgVarSpecs HmacDrbgFunSpecs
 Proof.
   start_function.
 
-  unfold md_relate; unfold convert_abs.
+  unfold md_relate(*; unfold convert_abs*).
   destruct r as [r1 [r2 internal_r]].
   simpl.
   rewrite REP_isptr; Intros. 
@@ -135,12 +124,11 @@ Proof.
   forward.
 
   rewrite INITNAME, CTX_Struct.
-  forward_call (internal_r, 32, key, kv).
+  forward_call (@inl _ (val * Z * list Z * val * block * int) (internal_r, 32, key, kv)). 
   forward.
 
-  unfold md_relate.
-  unfold convert_abs.
-  entailer!.
+  unfold md_relate; simpl. cancel.
+(*  unfold convert_abs.*)
 Qed.
 
 Lemma body_md_setup: semax_body HmacDrbgVarSpecs (malloc_spec::HmacDrbgFunSpecs)
@@ -149,8 +137,7 @@ Proof.
   start_function.
 
   forward_call (sizeof (Tstruct _hmac_ctx_st noattr)).
-  Intros. normalize. (*FAIL*)
-  apply extract_exists_pre. intros vret. (*SUCCESS*)
+  Intros vret. 
  
   forward_if (PROP () LOCAL (temp _sha_ctx vret; temp _md_info info; 
    temp _ctx c; temp _hmac h) 
